ulib/FStar.Relational.Comp.fst
@@ -1,67 +1,7 @@
-(*--build-config
-    options:;
-    other-files:FStar.List.Tot.fst FStar.FunctionalExtensionality.fst FStar.Set.fst FStar.Heap.fst FStar.ST.fst FStar.All.fst FStar.List.fst
-  --*)
-
-module FStar.Relational
-open FStar.Heap
-
-(* Relational Type constructor (Equivalent to pairs) *)
-type rel (a:Type) (b:Type) : Type =
-  | R : l:a -> r:b -> rel a b
-
-(* Some frequently used abbreviations *)
-type double (t:Type) = rel t t
-type eq (t:Type) = p:(double t){R.l p = R.r p}
-
-let twice x = R x x
-let tu = twice ()
-
-(* functions to lift normal functions to Relational functions *)
-val rel_map1T : ('a -> Tot 'b) -> (double 'a) -> Tot (double 'b)
-let rel_map1T f (R x1 x2)  = R (f x1) (f x2)
-
-val rel_map2T : ('a -> 'b -> Tot 'c) -> (double 'a) -> (double 'b) -> Tot (double 'c)
-let rel_map2T f (R x1 x2) (R y1 y2) = R (f x1 y1) (f x2 y2)
-
-val rel_map3T : ('a -> 'b -> 'c -> Tot 'd) -> (double 'a) -> (double 'b) -> (double 'c) -> Tot (double 'd)
-let rel_map3T f (R x1 x2) (R y1 y2) (R z1 z2) = R (f x1 y1 z1) (f x2 y2 z2)
-
-(* Some convenient arithmetic functions *)
-let op_Hat_Plus = rel_map2T (fun x y -> x + y)
-let op_Hat_Minus = rel_map2T (fun x y -> x - y)
-let op_Hat_Star = rel_map2T (fun x y -> x * y)
-let op_Hat_Slash = rel_map2T (fun x y -> x / y)
-
-(* Some convenient list functions *)
-val tl_rel: #a:Type -> l:double (list a){is_Cons (R.l l) /\ is_Cons (R.r l)}-> Tot (double (list a))
-let tl_rel #a (R (_::xs) (_::ys)) = R xs ys
-let cons_rel (R x y) (R xs ys) = R (x::xs) (y::ys) 
-(* Some convenient tuple functions *)
-let pair_rel (R a b) (R c d) = R (a,c) (b,d)
-let triple_rel (R a b) (R c d) (R e f) = R (a,c,e) (b,d,f)
-let fst_rel = rel_map1T fst 
-let snd_rel = rel_map1T snd 
- 
-(* Some convenient boolean functions *)
-let and_rel = rel_map2T (fun x y -> x && y)
-let or_rel = rel_map2T (fun x y -> x || y)
-let eq_rel = rel_map2T (fun x y -> x = y)
-
-(* Some convenient functions combining left and right side (for specification only) *)
-let and_irel (R a b) = a && b
-let or_irel (R a b) = a || b
-let eq_irel (R a b) = a = b
-
-(* Some convenient functions on heap (for specification) *)
-let sel_rel1 h r  = rel_map2T sel h (twice r)
-let sel_rel2 = rel_map2T sel
-let upd_rel = rel_map3T upd
-
-module FStar.Comp
+module FStar.Relational.Comp
 
 open FStar.Heap
-open FStar.Relational
+open FStar.Relational.Relational
 
 type heap2 = double heap
 
@@ -69,7 +9,7 @@ new_effect STATE2 = STATE_h heap2
 let st2_Pre = st_pre_h heap2
 let st2_Post (a:Type) = st_post_h heap2 a
 let st2_WP (a:Type) = st_wp_h heap2 a
-effect ST2 (a:Type) (pre:st2_Pre) (post: (heap2 -> st2_Post a)) =
+effect ST2 (a:Type) (pre:st2_Pre) (post: (heap2 -> Tot (st2_Post a))) =
     STATE2 a
       (fun (p:st2_Post a) (h:heap2) -> pre h /\ (forall a h1. (pre h /\ post h a h1) ==> p a h1)) (* WP *)
       (fun (p:st2_Post a) (h:heap2) -> (forall a h1. (pre h /\ post h a h1) ==> p a h1))          (* WLP *)
@@ -78,14 +18,15 @@ sub_effect
   DIV    ~> STATE2 = (fun (a:Type) (wp:pure_wp a) (p:st2_Post a) -> (fun h2 -> wp (fun a0 -> p a0 h2)))
 
 (* construct a st2_WP from 2 st_wps *)
-type comp (a:Type) (b:Type) (wp0:st_wp a) (wp1:st_wp b) (p:((rel a b) -> heap2 -> Type)) (h2:heap2) =
+val comp : (a:Type) -> (b:Type) -> (wp0:st_wp a) -> (wp1:st_wp b) -> Tot (st2_WP (rel a b)) 
+let comp a b wp0 wp1 p h2 =
     wp0 (fun y0 h0 ->
       wp1 (fun y1 h1 -> p (R y0 y1) (R h0 h1))
       (R.r h2))
     (R.l h2)
 
-assume val compose2: #a0:Type -> #b0:Type -> #wp0:(a0 -> st_wp b0) -> #wlp0:(a0 -> st_wp b0)
-                  -> #a1:Type -> #b1:Type -> #wp1:(a1 -> st_wp b1) -> #wlp1:(a1 -> st_wp b1)
+assume val compose2: #a0:Type -> #b0:Type -> #wp0:(a0 -> Tot (st_wp b0)) -> #wlp0:(a0 -> Tot (st_wp b0))
+                  -> #a1:Type -> #b1:Type -> #wp1:(a1 -> Tot (st_wp b1)) -> #wlp1:(a1 -> Tot (st_wp b1))
                   -> =c0:(x0:a0 -> STATE b0 (wp0 x0) (wlp0 x0))
                   -> =c1:(x1:a1 -> STATE b1 (wp1 x1) (wlp1 x1))
                   -> x: rel a0 a1
@@ -93,7 +34,7 @@ assume val compose2: #a0:Type -> #b0:Type -> #wp0:(a0 -> st_wp b0) -> #wlp0:(a0 
                             (comp b0 b1 (wp0 (R.l x)) (wp1 (R.r x)))
                             (comp b0 b1 (wlp0 (R.l x)) (wlp1 (R.r x)))
 
-val compose2_self : #a:Type -> #b:Type -> #wp:(a -> st_wp b) -> #wlp:(a -> st_wp b)
+val compose2_self : #a:Type -> #b:Type -> #wp:(a -> Tot (st_wp b)) -> #wlp:(a -> Tot (st_wp b))
                 -> =c:(x:a -> STATE b (wp x) (wlp x))
                 -> x: double a
                 -> STATE2 (double b)
@@ -124,42 +65,36 @@ assume val cross : #a:Type -> #b:Type -> #c:Type -> #d:Type
 
 
 (* Create a ST statment from a ST2 statement by projection *)
-type decomp_l (a0:Type) (a1:Type) (b0:Type) (b1:Type) (al:a0)
-            (wp:(rel a0 a1 -> st2_WP (rel b0 b1))) (p:b0 -> heap -> Type) (hl:heap) = 
+val decomp_l : (a0:Type) -> (a1:Type) -> (b0:Type) -> (b1:Type) -> (al:a0) -> (wp:(rel a0 a1 -> Tot (st2_WP (rel b0 b1)))) 
+	     -> Tot (st_wp_h heap b0)
+let decomp_l a0 a1 b0 b1 al wp = 
+  fun p hl ->
     (exists (ar:a1) (hr:heap).
       wp (R al ar) (fun y2 h2 -> p (R.l y2) (R.l h2))
          (R hl hr))
 
-type decomp_r (a0:Type) (a1:Type) (b0:Type) (b1:Type) (ar:a1)
-            (wp:(rel a0 a1 -> st2_WP (rel b0 b1))) (p:b1 -> heap -> Type) (hr:heap) =
+val decomp_r : (a0:Type) -> (a1:Type) -> (b0:Type) -> (b1:Type) -> (ar:a1) -> (wp:(rel a0 a1 -> Tot (st2_WP (rel b0 b1)))) 
+	     -> Tot (st_wp_h heap b1)
+let decomp_r a0 a1 b0 b1 ar wp =
+  fun p hr ->
     (exists (al:a0) (hl:heap).
       wp (R al ar) (fun y2 h2 -> p (R.r y2) (R.r h2))
          (R hl hr))
 
 assume val project_l : #a0:Type -> #b0:Type -> #a1:Type -> #b1:Type
-                    -> #wp:(rel a0 a1 -> st2_WP (rel b0 b1))
-                    -> #wlp:(rel a0 a1 -> st2_WP (rel b0 b1))
+                    -> #wp:(rel a0 a1 -> Tot (st2_WP (rel b0 b1)))
+                    -> #wlp:(rel a0 a1 -> Tot (st2_WP (rel b0 b1)))
                     -> =c:(x:rel a0 a1 -> STATE2 (rel b0 b1) (wp x) (wlp x))
                     -> x:a0
                     -> STATE b0 (decomp_l a0 a1 b0 b1 x wp)
                                 (decomp_l a0 a1 b0 b1 x wlp)
 
 assume val project_r : #a0:Type -> #b0:Type -> #a1:Type -> #b1:Type
-                    -> #wp:(rel a0 a1 -> st2_WP (rel b0 b1))
-                    -> #wlp:(rel a0 a1 -> st2_WP (rel b0 b1))
+                    -> #wp:(rel a0 a1 -> Tot (st2_WP (rel b0 b1)))
+                    -> #wlp:(rel a0 a1 -> Tot (st2_WP (rel b0 b1)))
                     -> =c:(x:rel a0 a1 -> STATE2 (rel b0 b1) (wp x) (wlp x))
                     -> x:a1
                     -> STATE b1 (decomp_r a0 a1 b0 b1 x wp)
                                 (decomp_r a0 a1 b0 b1 x wlp)
 
 
-module FStar.RelationalState
-open FStar.Comp
-open FStar.Relational
-open FStar.Heap
-
-(* Some convenient stateful functions *)
-let read_rel1 r = compose2_self read (twice r)
-let read_rel2 = compose2_self read
-let assign_rel1 r v = compose2_self (fun (a,b) -> write a b) (pair_rel (twice r) v)
-let assign_rel2 r v = compose2_self (fun (a,b) -> write a b) (pair_rel r v)
